Micro_Rust_Std_Lib/StdLib_All.thy
@@ -9,6 +9,7 @@ theory StdLib_All
     StdLib_Iterators
     StdLib_Logging
     StdLib_Option
+    StdLib_Range
     StdLib_References
     StdLib_Result
     StdLib_Slice
