Micro_Rust_Std_Lib/StdLib_Range.thy
@@ -1,0 +1,38 @@
+(* Copyright Amazon.com, Inc. or its affiliates. All Rights Reserved.
+   SPDX-License-Identifier: MIT *)
+
+(*<*)
+theory StdLib_Range                            
+  imports Crush.Crush Shallow_Micro_Rust.Range_Type
+begin
+(*>*)
+
+definition is_empty_contract :: \<open>'a::{ord} range \<Rightarrow> ('machine::{sepalg}, bool, 'abort) function_contract\<close> where
+  [crush_contracts]: \<open>is_empty_contract r \<equiv>
+    let pre  = \<top>;
+        post = \<lambda>res. \<langle>res \<longleftrightarrow> \<not>start r < end r\<rangle>
+     in make_function_contract pre post\<close>
+ucincl_auto is_empty_contract
+
+lemma is_empty_spec [crush_specs]:
+  shows \<open>\<Gamma> ; is_empty r \<Turnstile>\<^sub>F is_empty_contract r\<close>
+by (contract f: is_empty_def contract: is_empty_contract_def) crush_base
+
+definition contains_contract :: \<open>'a::{ord} range \<Rightarrow> 'a \<Rightarrow> ('machine::{sepalg}, bool, 'abort) function_contract\<close> where
+  [crush_contracts]: \<open>contains_contract r e \<equiv>
+    let pre  = \<top>;
+        post = \<lambda>res. \<langle>res \<longleftrightarrow> start r \<le> e \<and> e < end r\<rangle>
+     in make_function_contract pre post\<close>
+ucincl_auto contains_contract
+
+lemma contains_spec [crush_specs]:  
+  shows \<open>\<Gamma> ; contains r e \<Turnstile>\<^sub>F contains_contract r e\<close>
+by (contract f: contains_def contract: contains_contract_def) crush_base
+
+lemma range_into_list_make_range [micro_rust_simps]:
+  shows \<open>range_into_list (make_range s e) = list.map word_of_nat [unat s..<unat e]\<close>
+by (clarsimp simp add: range_into_list_def)
+
+(*<*)
+end
+(*>*)
